\begin{proof}
  We will show that $[X, Y]$ satisfies the Leibniz rule.
  Let $f, g \in \mathcal{F} M$.
  Then
  \begin{equation}
    X(Y(f g))
    = X(Y f \cdot g + f \cdot Y g)
    = X (Y f) \cdot g + Y f \cdot X g + X f \cdot Y g + f \cdot X (Y g).
  \end{equation}
  Analogously,
  \begin{equation}
    Y(X(f g))
    = Y (X f) \cdot g + X f \cdot Y g + Y f \cdot X g + f \cdot Y (X g).
  \end{equation}
  Hence,
  \begin{equation}
    [X, Y] (f g)
    = X(Y(f g)) - Y(X(f g))
    = X (Y f) \cdot g + f \cdot X (Y g) - Y (X f) \cdot g - f \cdot Y (X g)
    = [X, Y] f \cdot g + f \cdot [X, Y] g.
  \end{equation}
  Linearity of $[X, Y]$ is obvious.
  Hence, $[X, Y]$ is a vector field.
\end{proof}
