\begin{proposition}
  Let
    $R$ be a commutative ring with unity,
    $D \in \N$,
    $V$ be a free module over $R$ of dimension $D$,
    $e_0, ..., e_{D - 1}$ be a basis of $V$,
    $v_0, ..., v_{D - 1} \in V$ such that for $j = 0, ..., D - 1$,
  \begin{equation}
    v_j = \sum_{i = 0}^{D - 1} e_i A_{i, j}
  \end{equation}
  (in matrix form, $(v_0, ..., v_{D - 1}) = (e_0, ..., e_{D - 1}) A$).
  Then
  \begin{equation}
    v_0 \wedge ... \wedge v_{D - 1} = (\det A) e_0 \wedge ... \wedge e_{D - 1}.
  \end{equation}
  As a consequence, the matrix $A$ is a change of basis matrix if and only if
  $\det A$ is an invertible element of $R$
  (a nonzero element when $R$ is a field).
\end{proposition}
