\begin{proof}
  First, let $A$ be alternating.
  Then for any $a, b \in A$,
  \begin{equation}
    0 = \mu(a + b, a + b)
    = \mu(a, a) + \mu(a, b) + \mu(b, a) + \mu(b, b)
    = \mu(a, b) + \mu(b, a)
    \Rightarrow \mu(b, a) = - \mu(a, b).
  \end{equation}
  Conversely, let $A$ be anti-commutative. Taking $b = a$ in the definition
  leads to
  \begin{equation}
    \mu(a, a) = - \mu(a, a) \Rightarrow \mu(a, a) + \mu(a, a) = 0.
  \end{equation}
  Under the assumption of
  \Cref{equation:ring/characteristics_is_not_divisible_by_2},
  we conclude that $\mu(a, a) = 0$.
\end{proof}
