\begin{proof}
  Let $x, y, z \in A$.
  $[\cdot, \cdot]$ is alternating since $[x, x] = x x - x x = 0$.
  Next, we calculate
  \begin{equation}
    [x, [y, z]]
    = [x, y z - z y]
    = x (y z - z y) - (y z - z y) x
    = x y z - x z y - y z x + z y x.
  \end{equation}
  Similarly,
  $[y, [z, x]] = y z x - y x z - z x y + x z y$ and
  $[z, [x, y]] = z x y - z y x - x y z + y x z$.
  We can see that each of the six permutations of $(x, y, z)$ in products occurs
  twice with opposite signs, which means that their sum is zero.
  Hence, the Jacobi identity is also satisfied.
\end{proof}
