\begin{definition}
  Let
    $R$ be a commutative ring with unity,
    $V$ be an $R$-algebra with multiplication operation $[\cdot, \cdot]$.
  We say that $V$ is a \textbf{Lie algebra} if $[\cdot, \cdot]$ is alternating
  and satisfies the \textbf{Jacobi identity}: for any $x, y, z \in V$,
  \begin{equation}
    [x, [y, z]] + [y, [z, x]] + [z, [x, y]] = 0.
  \end{equation}
\end{definition}
\begin{proposition}
  Let
    $R$ be a commutative ring with unity,
    $V$ be an associative algebra over $R$.
  Define the \textbf{commutator}$ [\cdot, \cdot] \colon V \times V \to V$
  as follows: for any $x, y \in V$,
  \begin{equation}
    [x, y] := x y - y x.
  \end{equation}
  Then $(V, [\cdot, \cdot])$ is a Lie algebra.
  In particular, when $X$ is a module over $R$, $V := {\rm End}_R X$ is a Lie
  algebra with Lie bracket given by
  \begin{equation}
    [\varphi, \psi] := \varphi \circ \psi - \psi \circ \varphi,\
    \varphi, \psi \in {\rm End}_R X.
  \end{equation}
\end{proposition}
\begin{proof}
  Let $x, y, z \in A$.
  $[\cdot, \cdot]$ is alternating since $[x, x] = x x - x x = 0$.
  Next, we calculate
  \begin{equation}
    [x, [y, z]]
    = [x, y z - z y]
    = x (y z - z y) - (y z - z y) x
    = x y z - x z y - y z x + z y x.
  \end{equation}
  Similarly,
  $[y, [z, x]] = y z x - y x z - z x y + x z y$ and
  $[z, [x, y]] = z x y - z y x - x y z + y x z$.
  We can see that each of the six permutations of $(x, y, z)$ in products occurs
  twice with opposite signs, which means that their sum is zero.
  Hence, the Jacobi identity is also satisfied.
\end{proof}
\begin{definition}
  Let
    $R$ be a commutative ring with unity,
    $(V, [\cdot, \cdot]_V)$ and
    $(W, [\cdot, \cdot]_W)$ be Lie algebras over $R$,
    $\varphi \in \Hom_R(V, W)$.
  We say that $\varphi$ is a \textbf{Lie algebra homomorphism}
  if for any $u, v \in V$,
  \begin{equation}
    \varphi([u, v]_V) = [\varphi u, \varphi v]_W.
  \end{equation}
\end{definition}
\begin{definition}
  $R$ be a commutative ring with unity, $V$ be a Lie algebra over $R$.
  Define the \textbf{adjoint map}
  \begin{equation}
    {\rm adj} \colon V \to {\rm End}_R V,\
    {\rm adj}_x y := [x, y],\ x, y \in V.
  \end{equation}
\end{definition}
\begin{proposition}
  $R$ be a commutative ring with unity, $V$ be a Lie algebra over $R$.
  Then the adjoint map is a homorphism of Lie algebras, i.e.,
  for any $x, y \in V$,
  \begin{equation}
    {\rm adj}_{[x, y]}
    = [{\rm adj}_x, {\rm adj}_y]
    := {\rm adj}_x \circ {\rm adj}_y - {\rm adj}_y \circ {\rm adj}_x.
  \end{equation}
\end{proposition}
\begin{proof}
  Let $x, y, z \in V$.
  Then
  \begin{equation}
    \begin{split}
      [{\rm adj}_x, {\rm adj}_y] z
      & = ({\rm adj}_x \circ {\rm adj}_y - {\rm adj}_y \circ {\rm adj}_x) z
      = [x, [y, z]] - [y, [x, z]] \\
      & = [x, [y, z]] + [y, [z, x]]
      = - [z, [x, y]]
      = [[x, y], z]
      = {\rm adj}_{[x, y]} z.
      \qedhere
    \end{split}
  \end{equation}
\end{proof}
