\begin{discussion}
  \label{idec/heat_transport/discrete/mixed_weak_transient_solve_trapezoidal-discussion}
  We are going to derive a solution to
  \Cref{idec/heat_transport/discrete/mixed_weak_transient-formulation}
  using the trapezoidal rule for time integration.
  We will assume that the heat capacity $\pi_0$ is time-independent which will
  allow us to rearrange the time derivative:
  \begin{equation}
    C(v^d, \frac{\partial \tilde{u}^d} {\partial t})
    = \frac{d}{d t} C(v^d, \tilde{u}^d).
  \end{equation}
  For further simplicity we will also assume that all the rest input data (heat
  source, thermal conductivity, boundary conditions) are also time-independent.
  Denote $H := F + G$. We can then integrate the equation
  \begin{equation}
    B(v^d, q^{d - 1}) - \frac{d}{d t} C(v^d, \tilde{u}^d) = -F(v^d)
  \end{equation}
  with respect to $t$ in the interval $[\alpha, \beta] \subset I$ to get
  \begin{equation}
    B(v^d, \int_\alpha^\beta q^{d - 1}\, d t)
    - (C(v^d, \tilde{u}^d(\beta)) - C(v^d, \tilde{u}^d(\alpha)))
    = - (\beta - \alpha) F(v^d).
  \end{equation}
  If we partition $I$ into segements with size $\tau$ with moments of
  time $\{t_i := t_0 + \tau i\}_{i \geq 0}$, and if we denote
  $\{Q^s := q^{d - 1}(t_i)\}_{i \geq 0}$,
  $\{U^s := \tilde{u}^d(t_i)\}_{i \geq 0}$,
  we get
  \begin{equation}
    \frac{\tau}{2} (B(v^d, Q^s) + B(v^d, Q^{s + 1}))
    - (C(v^d, U^{s + 1}) - C(v^d, U^s))
    = - \tau F(v^d).
  \end{equation}
  The above equation is restated as
  \begin{equation}
    B(v^d, Q^{s + 1}) - \frac{2}{\tau} C(v^d, U^{s + 1})
    = - B(v^d, Q^s) - \frac{2}{\tau} C(v^d, U^s) - F(v^d).
  \end{equation}
  Define $H^s(v^d) := B(v^d, Q^s) + \frac{2}{\tau} C(v^d, U^s)$.
  We arrive at the following problem: find
  $\{(Q^s, U^s) \in C^{d - 1} K \times C^d K\}_{i \geq 0}$
  such that
  \begin{subequations}
    \begin{alignat}{4}
      & \forall r^{d - 1} [E T^{-1}] \in \Ker \tr_{\Gamma_N, D - 1}, \enspace
      && A(r^{d - 1}, Q^{s + 1}) + B^T(r^{d - 1}, U^{s + 1})
      && = G(r^{d - 1}), \enspace
      && i \geq 0, \\
%
      & \forall v^d [\Theta L^d] \in C^d K, \enspace
      && B(v^d, Q^{s + 1}) - \frac{2}{\tau} C(v^d, U^{s + 1})
      && = - H^s(v^d) - F(v^d), \enspace
      && i \geq 0, \\
%
      &
      && \tr_{\Gamma_N, d - 1} Q^s
      && = g_N^{d - 1}, \enspace
      && i > 0, \\
%
      &
      && Q^0
      % && = ((-1)^{d - 1} \kappa_{d - 1} \star_1 \delta_0)(u_0),
      && = {\rm flow}(u_0),
      && \\
%
      &
      && U^0
      && = \star_0 u_0.
      &&
    \end{alignat}
  \end{subequations}
  For $i > 0$ denote the unknown coefficients of $Q^s$ as
  $\{x^s_j\}_{j = 0}^{n_{d - 1} - 1}$, i.e.,
  \begin{equation}
    Q^s = \sum_{j = 0}^{n_{s - 1} - 1} x^s_j c^{d - 1, j},
  \end{equation}
  and the unknown coefficients of $U^s$ as
  $\{y^s_k\}_{k = 0}^{n_d - 1}$, i.e.,
  \begin{equation}
    U^s = \sum_{k = 0}^{n_d - 1} y^s_k c^{d, k}.
  \end{equation}
  Let
  \begin{subequations}
    \begin{alignat}{2}
      & J
      && := \set{i \in \{0, ..., n_{d - 1}\}}
        {c_{d - 1, i} \in (\Gamma_N)_{d - 1}}, \\
%
      & \overline{J}
      && := \{0, ..., n_{d - 1}\} \setminus J.
    \end{alignat}
  \end{subequations}
  Initil conditions give us $Q^0$ and $U^0$.
  Denoting the matrices ${\bf A}$, ${\bf B}$, ${\bf C}$ and vectors
  ${\bf Q}$, ${\bf U}$, ${\bf H}$, ${\bf F}$, ${\bf G}$
  of the corresponding operators in standard bases, we get the system
  for ${\bf Q}^s$ and ${\bf U}^s$, $s > 0$.
  \begin{subequations}
    \begin{alignat}{3}
      & \sum_{j = 0}^{n_{d - 1} - 1} {\bf A}_{i, j} {\bf Q}^{s + 1}_j
        - \sum_{k = 0}^{n_d - 1} ({\bf B}^T)_{i, k} {\bf U}^{s + 1}_k
      && = {\bf G}_i, \enspace
      && i \in \overline{J}, \\
%
      & \sum_{i = 0}^{n_{d - 1} - 1} {\bf B}_{k, i} {\bf Q}^{s +1}
        -\frac{2}{\tau} {\bf C} {\bf U}^{s + 1}
      && = - {\bf H}^s(v^d) - {\bf F}_k, \enspace
      && i \in \overline{J} \\
%
      & x_i
      && = g_N^{d - 1}(c{d - 1, i}), \enspace
      && i \in J.
    \end{alignat}
  \end{subequations}
  This leads to the follwoing system of equations for any $s \in \N$:
  \begin{subequations}
    \begin{alignat}{3}
      & \sum_{j \in \overline{J}} {\bf A}_{i, j} {\bf Q}^{s + 1}_j
        - \sum_{k = 0}^{n_d - 1} ({\bf B}^T)_{i, k} {\bf U}^{s + 1}_k
      && = {\bf G}_i -
        \sum_{j \in J} {\bf A}_{i, j} g_N^{d - 1}(c_{d - 1, j}), \enspace
      && i \in \overline{J}, \\
%
      & \sum_{i \in J} {\bf B}_{k, i} {\bf Q}^{s + 1}_i
        - \sum_{l = 0}^{n_d - 1}
          \frac{2}{\tau}{\bf C}_{k, l} {\bf U}^{s + 1}_l
      && = - \overline{\bf H}({\bf U}^s, {\bf U}^s)_k - {\bf F}_k
        - \sum_{i \in J} {\bf B}_{k, i} g_N^{d - 1}(c_{d - 1, i}), \enspace
      && i \in \overline{J}.
    \end{alignat}
  \end{subequations}
  Define matrices $\overline{\bf A}$, $\overline{\bf B}$,
  vectors, $\overline{\bf F}$, $\overline{\bf G}$,
  and unknowns (for $s \in \N$) $\overline{\bf Q}^{s + 1}$ in the obvious way.
  For any $s \in \N$ we get the mixed system
  \begin{subequations}
    \begin{alignat}{2}
      & \overline{\bf A}\, \overline{\bf Q}^{s + 1}
        + \overline{\bf B}^T {\bf U}^{s + 1}
      && = \overline{\bf G}, \\
%
      & \overline{\bf B}\, \overline{\bf Q}^{s + 1}
        - \frac{2}{\tau} {\bf C} {\bf U}^{s + 1}
      && = - {\bf H}({\bf Q}^s, {\bf U}^s) - \overline{\bf F}.
    \end{alignat}
  \end{subequations}
  We can solve for $\overline{\bf Q}^{s + 1}$, $s \in \N$ as follows:
  \begin{equation}
    \overline{\bf Q}^{s + 1}
    = \overline{\bf A}^{-1}
      (\overline{\bf G} - \overline{\bf B}^T {\bf U}^{s + 1}).
  \end{equation}
  Hence,
  \begin{equation}
    - {\bf H}({\bf Q}^s, {\bf U}^s) - \overline{\bf F}
    = \overline{\bf B}\, \overline{\bf Q}^{s + 1}
      - \frac{2}{\tau} {\bf C} {\bf U}^{s + 1}
    = \overline{\bf B}\, \overline{\bf A}^{-1}
      (\overline{\bf G} - \overline{\bf B}^T {\bf U}^{s + 1})
      - \frac{2}{\tau} {\bf C} {\bf U}^{s + 1},
  \end{equation}
  which translates to
  \begin{equation}
    (\overline{\bf B}\, \overline{\bf A}^{-1} \overline{\bf B}^T
      + \frac{2}{\tau} {\bf C}) {\bf U}^{s + 1}
    = \overline{\bf B} \overline{\bf A}^{-1} \overline{\bf G}
      + \overline{\bf F} + {\bf H}({\bf Q}^s, {\bf U}^s).
  \end{equation}
  Define the left-hand side matrix ${\bf N}_\tau \in M_{n_d \times n_d}(\R)$,
  \begin{equation}
    {\bf N}_\tau
    := \overline{\bf B}\, \overline{\bf A}^{-1} \overline{\bf B}^T
      + \frac{2}{\tau} {\bf C},
  \end{equation},
  and the constant right-hand side vector ${\bf Z} \in \R^{n_d}$,
  \begin{equation}
    {\bf Z}
    := \overline{\bf B} \overline{\bf A}^{-1} \overline{\bf G}
      + \overline{\bf F}
  \end{equation}
  This leads to the following linear $n_d \times n_d$ system:
  \begin{equation}
    {\bf N}_\tau {\bf U}^{s + 1}
    = {\bf Z} + {\bf B} {\bf Q}^s + \frac{2}{\tau} {\bf C} {\bf U}^s.
  \end{equation}
  We can apply the Cholesky decomposition to the left-hand side to arrive at
  the following algorithm.
\end{discussion}
