\begin{definition}
  Let $V$ be a vector space over $\R$.
  An inner product on $V$ is a function $g \colon V \times V \to \R$ that is:
  \begin{enumerate}
    \item
      bilinear, i.e., for all $\lambda, \mu \in \R$, $u, v, w \in V$:
      \begin{equation}
        g(\lambda u + \mu v, w) = \lambda g(u, w) + \mu g(v, w),\
        g(w, \lambda u + \mu v) = \lambda g(w, u) + \mu g(w, v);
      \end{equation}
    \item
      symmetric, i.e., for all $u, v \in V$,
      \begin{equation}
        g(u, v) = g(v, u);
      \end{equation}
    \item
      positive definite: for all $v \in V \setminus \{0\}$,
      \begin{equation}
        g(v, v) > 0.
      \end{equation}
  \end{enumerate}
  If $g$ is an inner product on $V$, the pair $(V, g)$ is called an
  \textbf{real inner product space}.
\end{definition}
\begin{notation}
  Let $R$ be a commutative ring with unity and $V$ be a module over $R$.
  Denote by $V^*$ the \textbf{dual space} of $V$:
  \begin{equation}
    V^* := \Hom(V, R).
  \end{equation}
\end{notation}
\begin{proposition}
  Let $(V, g)$ be a finite-dimensional real inner product space.
  Define the map $\tilde{g} \colon V \to V^*$ as follows: for any $v \in V$,
  \begin{equation}
    \tilde{g}(v) := (w \in V \mapsto g(v, w)).
  \end{equation}
  Then $\tilde{g}$ is an isomorphism.
\end{proposition}
\begin{definition}
  Let
    $d \in \N$,
    $(V, g)$ be a real inner product space of dimension $d$,
    $e = \{e_0, ..., e_{d - 1}\}$ be a basis of $V$.
  We say that $e$ is an \textbf{orthogonal basis} if any two disjoint elements
  are orthogonal, i.e., for all $i, j \in \{0, ..., d - 1\}$,
  if $i \neq j$, then
  \begin{equation}
    g(e_i, e_j) = 0.
  \end{equation}
  The basis $e$ is called \textbf{orthonormal}, if it is orthogonal and
  for any $i \in \{0, ..., d - 1\}$,
  \begin{equation}
     g(e_i, e_i) = 1.
  \end{equation}
  An equivalent way of saying that $e$ is orthonormal is by using the Kronecker
  delta symbol: for all $i, j \in \{0, ..., d - 1\}$,
  \begin{equation}
    g(e_i, e_j) = \delta_{i, j} :=
    \begin{cases}
      0, & \text{if $i \neq j$} \\
      1, & \text{if $i = j$}
    \end{cases}.
  \end{equation}
\end{definition}
